platform/cito/MakeADT.v
@@ -292,12 +292,12 @@ Module Make (Import E : ADT) (Import M : RepInv E).
   Qed.
 
   Lemma store_pair_inl_fwd : forall h w v,
-    is_heap (store_pair h (w, inl v)) ===> is_heap h.
+    is_heap (store_pair h (w, SCA _ v)) ===> is_heap h.
     intros; apply Himp_refl.
   Qed.
 
   Lemma store_pair_inl_bwd : forall h w v,
-    is_heap h ===> is_heap (store_pair h (w, inl v)).
+    is_heap h ===> is_heap (store_pair h (w, SCA _ v)).
     intros; apply Himp_refl.
   Qed.
 
@@ -308,7 +308,7 @@ Module Make (Import E : ADT) (Import M : RepInv E).
 
   Lemma store_pair_inr_fwd : forall h w v,
     ~WordMap.In w h
-    -> is_heap (store_pair h (w, inr v)) ===> rep_inv w v * is_heap h.
+    -> is_heap (store_pair h (w, ADT v)) ===> rep_inv w v * is_heap h.
     unfold store_pair; simpl.
     intros.
     unfold is_heap at 1.
@@ -351,7 +351,7 @@ Module Make (Import E : ADT) (Import M : RepInv E).
 
   Lemma store_pair_inr_bwd : forall h w v,
     ~WordMap.In w h
-    -> rep_inv w v * is_heap h ===> is_heap (store_pair h (w, inr v)).
+    -> rep_inv w v * is_heap h ===> is_heap (store_pair h (w, ADT v)).
     unfold store_pair; simpl.
     intros.
     unfold is_heap at 2.
@@ -512,14 +512,14 @@ Module Make (Import E : ADT) (Import M : RepInv E).
     match goal with
       | [ |- Regs ?a ?b = fst (decide_ret ?X ?Y) ] =>
         let w := fresh "w" in evar (w : W); let w' := eval unfold w in w in clear w;
-          equate X (Regs a b); equate Y (@inl _ ADTValue w'); reflexivity
+          equate X (Regs a b); equate Y (@SCA ADTValue w'); reflexivity
     end.
 
   Ltac returnAdt1 :=
     match goal with
       | [ |- Regs ?a ?b = fst (decide_ret ?X ?Y) ] =>
         let a := fresh "a" in evar (a : ADTValue); let a' := eval unfold a in a in clear a;
-          equate X (Regs a b); equate Y (@inr W _ a'); reflexivity
+          equate X (Regs a b); equate Y (ADT a'); reflexivity
     end.
 
   Ltac returnSomething := intuition; (cbv beta; simpl;
